Added a loop to ArrayTest

platform/tests/ArrayTest.v
@@ -1,4 +1,4 @@
-Require Import AutoSep.
+Require Import Arith AutoSep.
 
 
 Definition readS := SPEC("arr", "pos") reserving 0
@@ -11,16 +11,193 @@ Definition writeS := SPEC("arr", "pos", "val") reserving 0
   PRE[V] array8 arr (V "arr") * [| V "pos" < $(length arr) |]
   POST[_] array8 (Array8.upd arr (V "pos") (WtoB (V "val"))) (V "arr").
 
+Definition inc1 (b : B) : B := WtoB (BtoW b ^+ $1).
+Definition inc := map inc1.
+
+Definition incS := SPEC("arr", "len") reserving 2
+  Al arr,
+  PRE[V] array8 arr (V "arr") * [| V "len" = length arr |] * [| goodSize (length arr) |]
+  POST[_] array8 (inc arr) (V "arr").
+
 Definition m := bmodule "array" {{
-  bfunction "read"("arr", "pos") [readS]
+  (*bfunction "read"("arr", "pos") [readS]
     "arr" <-*8 "arr" + "pos";;
     Return "arr"
   end with bfunction "write"("arr", "pos", "val") [writeS]
     "arr" + "pos" *<-8 "val";;
     Return 0
+  end with*) bfunction "inc"("arr", "len", "i", "tmp") [incS]
+    "i" <- 0;;
+
+    [Al arr,
+      PRE[V] array8 arr (V "arr") * [| V "len" = length arr |] * [| goodSize (length arr) |]
+        * [| (V "i" <= $(length arr))%word |]
+      POST[_] Ex arr', array8 arr' (V "arr") * [| length arr' = length arr |]
+        * [| forall j, (j < wordToNat (V "i"))%nat -> Array8.selN arr' j = Array8.selN arr j |]
+        * [| forall j, (j >= wordToNat (V "i"))%nat -> Array8.selN arr' j = inc1 (Array8.selN arr j) |] ]
+    While ("i" < "len") {
+      "tmp" <-*8 "arr" + "i";;
+      "tmp" <- "tmp" + 1;;
+      "arr" + "i" *<-8 "tmp";;
+      "i" <- "i" + 1
+    };;
+
+    Return 0
   end
 }}.
 
+Hint Rewrite roundTrip_0 : N.
+
+Lemma zero_le : forall w : W, natToW 0 <= w.
+  intros; nomega.
+Qed.
+
+Hint Immediate zero_le.
+
+Lemma length_upd' : forall v bs p,
+  length (Array8.updN bs p v) = length bs.
+  induction bs; simpl; intuition.
+  destruct p; simpl; intuition.
+Qed.
+
+Lemma length_upd : forall p v bs,
+  length (Array8.upd bs p v) = length bs.
+  intros; apply length_upd'.
+Qed.
+
+Hint Rewrite length_upd : sepFormula.
+
+Lemma next' : forall (i : W),
+  (exists len' : W, (wordToNat i < wordToNat len')%nat)
+  -> wordToNat (i ^+ $(1)) = wordToNat i + 1.
+  destruct 1; erewrite next; eauto.
+  instantiate (1 := x); nomega.
+Qed.
+
+Hint Rewrite next' using (eexists; eassumption) : N.
+
+Lemma next : forall (i : W),
+  (exists len' : W, i < len')
+  -> wordToNat (i ^+ $(1)) = wordToNat i + 1.
+  destruct 1; eapply next'; eauto.
+  pre_nomega; eauto.
+Qed.
+
+Hint Rewrite next using (eexists; eassumption) : sepFormula.
+
+Lemma increment : forall (i len len' : W),
+  i < len
+  -> len = len'
+  -> i ^+ $1 <= len'.
+  intros; subst; pre_nomega; nomega.
+Qed.
+
+Hint Immediate increment.
+
+Lemma wordToNat_eq : forall sz (u v : word sz),
+  wordToNat u = wordToNat v
+  -> u = v.
+  intros; apply (f_equal (@natToWord sz)) in H;
+    repeat rewrite natToWord_wordToNat in H; auto.
+Qed.
+
+Lemma squeeze : forall (len i len' : W),
+  len <= i
+  -> len = len'
+  -> i <= len'
+  -> len' = i.
+  intros; subst; apply wordToNat_eq; nomega.
+Qed.
+
+Lemma inc_nil : inc nil = nil.
+  auto.
+Qed.
+
+Hint Rewrite inc_nil app_nil_r : sepFormula.
+Hint Rewrite wordToNat_natToWord_idempotent using assumption : sepFormula.
+
+Lemma determine_inc : forall arr arr',
+  length arr' = length arr
+  -> (forall j, Array8.selN arr' j = inc1 (Array8.selN arr j))
+  -> arr' = inc arr.
+  induction arr; destruct arr'; simpl; intuition; f_equal.
+  apply (H0 O).
+  apply IHarr; auto.
+  intro j; apply (H0 (S j)).
+Qed.
+
+Lemma selN_updN_eq : forall v ls p,
+  (p < length ls)%nat
+  -> Array8.selN (Array8.updN ls p v) p = v.
+  induction ls; simpl; intuition.
+  destruct p; simpl; intuition.
+Qed.
+
+Lemma selN_updN_ne : forall v ls p p',
+  (p < length ls)%nat
+  -> p <> p'
+  -> Array8.selN (Array8.updN ls p v) p' = Array8.selN ls p'.
+  induction ls; simpl; intuition.
+  destruct p, p'; simpl; intuition.
+Qed.
+
+Lemma selN_upd_eq : forall v ls p,
+  goodSize (length ls)
+  -> p < natToW (length ls)
+  -> Array8.selN (Array8.upd ls p v) (wordToNat p) = v.
+  unfold Array8.upd; intros; apply selN_updN_eq; nomega.
+Qed.
+
+Lemma selN_upd_ne : forall v ls p p',
+  goodSize (length ls)
+  -> p < natToW (length ls)
+  -> wordToNat p <> p'
+  -> Array8.selN (Array8.upd ls p v) p' = Array8.selN ls p'.
+  unfold Array8.upd; intros; apply selN_updN_ne; auto; nomega.
+Qed.
+
+Hint Resolve selN_upd_ne selN_upd_eq.
+
+Hint Extern 1 (not (@eq nat _ _)) => omega.
+Hint Extern 1 (_ < _) => congruence.
+
+Lemma selN_oob : forall ls i,
+  (i >= length ls)%nat
+  -> Array8.selN ls i = wzero _.
+  induction ls; simpl; intuition.
+  destruct i; simpl; intuition.
+Qed.
+
+Lemma final_bound : forall (len i : W) len' j,
+  goodSize len'
+  -> len <= i
+  -> len = natToW len'
+  -> i <= natToW len'
+  -> (j >= wordToNat i)%nat
+  -> (j >= len')%nat.
+  intros.
+  assert (natToW len' = i) by eauto using squeeze.
+  subst.
+  rewrite wordToNat_natToWord_idempotent in H3; auto.
+Qed.
+
+Hint Resolve final_bound.
+
+Ltac useHyp := match goal with
+                 | [ H : forall j : nat, _ |- _ ] => rewrite H by omega
+               end.
+
+Ltac finish :=
+  match goal with
+    | [ |- _ ^+ _ <= _ ] => eauto
+    | [ |- himp _ (array8 ?A _) (array8 ?B _) ] =>
+      replace B with A by eauto using determine_inc; reflexivity
+    | _ => solve [ useHyp; auto ]
+    | _ => solve [ rewrite selN_oob; eauto ]
+    | [ H : (?N >= ?M)%nat |- _ ] => destruct (eq_nat_dec N M); subst;
+      useHyp; auto; rewrite selN_upd_ne; auto
+  end.
+
 Theorem ok : moduleOk m.
-  vcgen; abstract sep_auto.
+  vcgen; abstract (sep_auto; finish).
 Qed.
